Phi_Examples/PhiEx_Slice.thy
@@ -40,19 +40,29 @@ proc qsort:
         $d \<leftarrow> $d + 1
       \<medium_right_bracket>
       \<medium_left_bracket> \<medium_right_bracket> ;;
-thm useful 
+
     \<medium_right_bracket> ;;
 
     (*readers may inspect \<open>thm useful\<close> to look the contextual facts*)
     (* thm useful *)
     qsort ($i, $d) ;;
-    qsort ($i + $d, $len - $d) ;;
-         
-    holds_fact take_and_drop[useful]: \<open>(\<forall>x\<in>set (drop d l'). l ! (len - 1) < x) \<and>
-                                       (\<forall>x\<in>set (take d l'). x \<le> l ! (len - 1))\<close> 
-    note sorted_append[simp] ;;
+    qsort ($i + $d, $len - $d) thm useful  ;;
+        
+    holds_fact t1: \<open>(\<forall>x\<in>set (drop d l'). l ! (len - 1) < x)\<close>
+           and t2: \<open>(\<forall>x\<in>set (take d l'). x \<le> l ! (len - 1))\<close>
+           and t4[simp]: \<open>set l'b = set (drop d l')\<close>
+    from \<open>mset (take d l') = mset l'a\<close> have t3[simp]: \<open>set l'a = set (take d l')\<close> by auto_sledgehammer
+;; (* 
+    holds_fact t1: \<open>set (drop (length l'a) l') = set l'b\<close>
+           and t2: \<open>set (take (length l'a) l') = set l'a\<close>
+           and t3: \<open>\<forall>j < length l'a. \<exists>k<length l'a. l'a ! j = l' ! k\<close>
+thm useful
+ ;; *)
+    note [\<phi>sledgehammer_simps] = sorted_append  ;;
 
-    return
+    return (*certified apply auto
+apply (auto_sledgehammer)[1]
+apply (auto_sledgehammer)[1]*)
 
   \<medium_right_bracket>
 \<medium_right_bracket> .
