Phi_StdLib/PhiStd_Loop.thy
@@ -46,6 +46,7 @@ proc (nodef) map_list_loop:
   input  \<open>X\<heavy_comma> l \<Ztypecolon> T\<heavy_comma> len \<Ztypecolon> \<v>\<a>\<l> \<nat>('b)\<close>
   output \<open>X\<heavy_comma> map_index f l \<Ztypecolon> T\<close> 
 \<medium_left_bracket>
+  note list_eq_iff_nth_eq [\<phi>sledgehammer_simps];;
   var i \<leftarrow> \<open>0 \<Ztypecolon> \<nat>('b)\<close> ;;
   while \<open>X\<heavy_comma> l' \<Ztypecolon> T\<heavy_comma> i \<Ztypecolon> \<v>\<a>\<r>[i] \<nat>('b) \<s>\<u>\<b>\<j> l' i.
            Inv: (i \<le> length l \<and> length l' = len \<and>
@@ -57,7 +58,7 @@ proc (nodef) map_list_loop:
       body ($i)
       apply_rule ToA_Mapper_backward[OF map[where i1=i]]
               is \<open>list_upd_map i (f i) l'\<close> certified using ToA_Mapper_f_expn[OF map[where i1=i]] by auto_sledgehammer ;;
-      $i \<leftarrow> $i + \<open>1 \<Ztypecolon> \<nat>('b)\<close>
+      $i \<leftarrow> $i + \<open>1 \<Ztypecolon> \<nat>('b)\<close> 
     \<medium_right_bracket> ;;
 \<medium_right_bracket> .
 
